SimAsm/State2.thy
@@ -58,4 +58,6 @@ end (* context state *)
 interpretation interpreted: state "\<lambda>x a. Some ()" "\<lambda>s a b. s" "(\<lambda>x. ()) :: unit \<Rightarrow> unit" "\<lambda>s f. s"
   unfolding state_def by auto
 
+
+
 end
